Split stlc in multiple files

theories/stlc.v
@@ -1,5 +1,4 @@
-From stdpp Require Export decidable list.
-Import Nat.
+Require Export stlc_types.
 
 
 (***********************************)
@@ -7,499 +6,179 @@ Import Nat.
 (***********************************)
 
 
-(**************)
-(** ** Syntax *)
-(**************)
-
-(** Global notation declarations. *)
-Declare Scope stlc_scope.
-Delimit Scope stlc_scope with stlc.
-Open Scope stlc_scope.
-Declare Custom Entry stlc_ty.
-
-
-(** Reverse list interface *)
-Module Type RLIST.
-  Parameter rlist : Type -> Type.
-
-  Parameter rlength : forall {A}, rlist A -> nat.
-
-  Declare Instance rlist_lookup {A} : Lookup nat A (rlist A).
-  Axiom is_Some_lookup : forall {A} (c : rlist A) n,
-    is_Some (c !! n) <-> n < rlength c.
-
-  Parameter rcons : forall {A}, rlist A -> A -> rlist A.
-  Axiom rlength_rcons :
-    forall {A} (c : rlist A) t, rlength (rcons c t) = S (rlength c).
-  Axiom lookup_rcons_eq : forall {A} (c : rlist A) t n,
-    n = rlength c -> rcons c t !! n = Some t.
-  Axiom lookup_rcons_lt : forall {A} (c : rlist A) t n,
-    n < rlength c -> rcons c t !! n = c !! n.
-
-  (** Build a list from its length and its (total) lookup function *)
-  Parameter build_rlist : forall {A}, nat -> (nat -> A) -> rlist A.
-  Axiom rlength_build_rlist : forall {A} n (f : nat -> A),
-    rlength (build_rlist n f) = n.
-  Axiom lookup_build_rlist : forall {A} l (f : nat -> A) n,
-    n < l -> build_rlist l f !! n = Some (f n).
-
-  Declare Instance rlist_fmap : FMap rlist.
-  Axiom lookup_fmap : forall {A} {B} (f : A -> B) (l : rlist A) n,
-    (f <$> l) !! n = f <$> l !! n.
-End RLIST.
-
-Module RlistTheories (Rlist : RLIST).
-  Export Rlist.
-
-  Notation "l +: e" := (rcons l e) (at level 50) : stlc_scope.
-  Notation "|( c )|" := (rlength c) : stlc_scope.
-
-
-  Definition lookup_default {A} d n (c : rlist A) : A :=
-    match c !! n with
-    | None => d
-    | Some x => x
-    end.
-
-  Theorem lookup_None1 {A} (c : rlist A) n :
-    n >= |(c)| -> c !! n = None.
-  Proof.
-    intros H.
-    destruct (c !! n) eqn : E; [|reflexivity].
-    assert (n < |(c)|); [|lia].
-    apply is_Some_lookup.
-    econstructor. eassumption.
-  Qed.
-
-  Theorem lookup_None2 {A} (c : rlist A) n :
-    c !! n = None -> n >= |(c)|.
-  Proof.
-    intros H.
-    destruct (decide (n < |(c)|)); [|lia].
-    apply is_Some_lookup in l. destruct l. now rewrite H in H0.
-  Qed.
-
-  Theorem lookup_rcons_gt : forall {A} (c : rlist A) t n,
-    n > |(c)| -> rcons c t !! n = None.
-  Proof.
-    intros. apply lookup_None1.
-    rewrite rlength_rcons. lia.
-  Qed.
-
-  Inductive lookup_rcons_cases {A} (c : rlist A) t n : Prop :=
-    | lookup_rcons_cases_lt (_ : n < |(c)|) (_ : (c +: t) !! n = c !! n)
-    | lookup_rcons_cases_eq (_ : n = |(c)|) (_ : (c +: t) !! n = Some t)
-    | lookup_rcons_cases_gt (_ : n > |(c)|) (_ : (c +: t) !! n = None).
-
-  Theorem lookup_rcons_spec {A} (c : rlist A) t n : lookup_rcons_cases c t n.
-  Proof.
-    destruct (lt_total n |(c)|) as [H | [H | H]].
-    - apply lookup_rcons_cases_lt; [assumption|].
-      now apply lookup_rcons_lt.
-    - apply lookup_rcons_cases_eq; [assumption|].
-      now apply lookup_rcons_eq.
-    - apply lookup_rcons_cases_gt; [assumption|].
-      now apply lookup_rcons_gt.
-  Qed.
-
-  Ltac lookup_rcons_spec c t n H E :=
-    destruct (lookup_rcons_spec c t n) as [H E | H E | H E]; rewrite E in *.
-
-  Theorem is_Some_rlength {A B} (l : rlist A) (h : rlist B) :
-    (forall n, is_Some (l !! n) <-> is_Some (h !! n)) ->
-    |(l)| = |(h)|.
-  Proof.
-    intros H. destruct (lt_total |(l)| |(h)|) as [E|[L|G]]; try assumption.
-    - apply is_Some_lookup in E. apply H in E.
-      apply is_Some_lookup in E. lia.
-    - apply is_Some_lookup in G. apply H in G.
-      apply is_Some_lookup in G. lia.
-  Qed.
-
-  Theorem rlength_fmap : forall {A} {B} (f : A -> B) l,
-    |(f <$> l)| = |(l)|.
-  Proof.
-    intros. apply is_Some_rlength.
-    intros. rewrite lookup_fmap. apply fmap_is_Some.
-  Qed.
-End RlistTheories.
-
-
-Module RlistList <: RLIST.
-  Definition rlist := list.
-  Definition rlength := @length.
-  Definition rcons {A} l (e : A) := l ++ [e].
-
-  Theorem rlength_rcons {A} :
-    forall (c : rlist A) t, length (rcons c t) = S (length c).
-  Proof.
-    intros. unfold rcons.
-    rewrite length_app. simpl. lia.
-  Qed.
-
-  Instance rlist_lookup {A} : Lookup nat A (rlist A) := list_lookup.
-
-  Theorem lookup_rcons_lt : forall {A} (c : rlist A) t n,
-    n < length c -> rcons c t !! n = c !! n.
-  Proof.
-    intros. unfold rcons.
-    now rewrite @lookup_app_l.
-  Qed.
-
-  Theorem is_Some_lookup {A} :
-    forall (c : rlist A) n, is_Some (c !! n) <-> n < length c.
-  Proof. apply lookup_lt_is_Some. Qed.
-
-  Theorem lookup_rcons_eq : forall {A} (c : rlist A) t n,
-    n = length c -> rcons c t !! n = Some t.
-  Proof.
-    intros. unfold rcons.
-    rewrite @lookup_app_r; [|lia].
-    subst. now rewrite sub_diag.
-  Qed.
-
-  Fixpoint build_rlist {A} n f : rlist A :=
-    match n with
-    | 0 => []
-    | S n => rcons (build_rlist n f) (f n)
-    end.
-
-  Theorem rlength_build_rlist : forall {A} n (f : nat -> A),
-    length (build_rlist n f) = n.
-  Proof.
-    intros. induction n; [reflexivity|].
-    simpl. unfold rcons.
-    rewrite length_app. rewrite IHn. simpl. lia.
-  Qed.
-
-  Theorem lookup_build_rlist : forall {A} n (f : nat -> A) x,
-    x < n -> build_rlist n f !! x = Some (f x).
-  Proof.
-    intros. induction n; [lia|].
-    simpl. unfold rcons.
-    destruct (decide (x = n)).
-    - subst. rewrite @lookup_app_r; rewrite rlength_build_rlist; [|lia].
-      now rewrite sub_diag.
-    - rewrite @lookup_app_l.
-      + apply IHn. lia.
-      + rewrite rlength_build_rlist. lia.
-  Qed.
-
-  Instance rlist_fmap : FMap rlist := list_fmap.
-
-  Theorem lookup_fmap : forall {A} {B} (f : A -> B) (l : rlist A) n,
-    (f <$> l) !! n = f <$> l !! n.
-  Proof. intros. apply list_lookup_fmap. Qed.
-End RlistList.
-
-
-(** *** Types *)
-
-(** Interface for the types of stlc.  There must be a type for propositions and
-    an arrow type. *)
-Module Type TY.
-  Parameter ty : Set.
-  Parameter ty_prp : ty.
-  Parameter ty_arr : ty -> ty -> ty.
-
-  Declare Instance eq_ty_dec : EqDecision ty.
-
-  Parameter ty_rec :
-    forall P : ty -> Set,
-    P ty_prp ->
-    (forall t, P t -> forall s, P s -> P (ty_arr t s)) ->
-    (forall t, P t) ->
-    forall t, P t.
-
-  Axiom ty_rec_prp : forall P p a d, ty_rec P p a d ty_prp = p.
-  Axiom ty_rec_arr : forall P p a d A B,
-    ty_rec P p a d (ty_arr A B) = a _ (ty_rec P p a d A) _ (ty_rec P p a d B).
-  Axiom ty_rec_neq : forall P p a d t,
-    t <> ty_prp -> (forall A B, t <> ty_arr A B) -> ty_rec P p a d t = d t.
-
-  Axiom ty_ind :
-    forall P : ty -> Prop,
-    P ty_prp ->
-    (forall t, P t -> forall s, P s -> P (ty_arr t s)) ->
-    (forall t, t <> ty_prp -> (forall A B, t <> ty_arr A B) -> P t) ->
-    forall t, P t.
-End TY.
-
-Module TyTheories (Ty : TY) (Rlist : RLIST).
-  Export Ty.
-  Module RlistTheories := RlistTheories Rlist.
-  Export RlistTheories.
-
-  Notation "-[ x ]-" := x (x custom stlc_ty) : stlc_scope.
-  Notation "x" := x (in custom stlc_ty at level 0, x global) : stlc_scope.
-  Notation "A -> B" := (ty_arr A B)
-    (in custom stlc_ty at level 99, right associativity) : stlc_scope.
-  Notation "( t )" := t
-    (in custom stlc_ty at level 0, t custom stlc_ty) : stlc_scope.
-  Notation "'o'" := ty_prp (in custom stlc_ty at level 0) : stlc_scope.
-
-
-  Create HintDb ty.
-  Hint Rewrite ty_rec_prp ty_rec_arr : ty.
-  Ltac ty_simpl := simpl in *; autorewrite with ty in *.
-
-
-  Definition ty_match {T : Set} p a d : ty -> T :=
-    ty_rec (fun _ => T) p (fun A _ B _ => a A B) (fun _ => d).
-
-  Theorem ty_arr_inj A B C D :
-    ty_arr A B = ty_arr C D -> A = C /\ B = D.
-  Proof.
-    intros H. split.
-    - apply (f_equal (ty_rec _ ty_prp (fun A _ B _ => A)
-        (fun _ => ty_prp))) in H.
-      now ty_simpl.
-    - apply (f_equal (ty_rec _ ty_prp (fun A _ B _ => B)
-        (fun _ => ty_prp))) in H.
-      now ty_simpl.
-  Qed.
-
-
-  Definition context := rlist ty.
-End TyTheories.
-
-
-Module TyChurch <: TY.
-  Inductive tyc : Set :=
-    | tyc_prp : tyc
-    | tyc_arr : tyc -> tyc -> tyc
-    | tyc_obj : tyc.
-
-  Definition ty := tyc.
-  Definition ty_prp := tyc_prp.
-  Definition ty_arr := tyc_arr.
-
-  Instance eq_ty_dec : EqDecision ty.
-  Proof. solve_decision. Defined.
-
-  Definition ty_rec :
-    forall P : ty -> Set,
-    P ty_prp ->
-    (forall t, P t -> forall s, P s -> P (ty_arr t s)) ->
-    (forall t, P t) ->
-    forall t, P t :=
-    fun P p a d => tyc_rec P p a (d tyc_obj).
-
-  Theorem ty_ind :
-    forall P : ty -> Prop,
-    P ty_prp ->
-    (forall t, P t -> forall s, P s -> P (ty_arr t s)) ->
-    (forall t, t <> ty_prp ->
-      (forall A B, t <> ty_arr A B) -> P t) ->
-    forall t, P t.
-  Proof. intros ? ? ? ? t. induction t; auto. Qed.
-
-  Theorem ty_rec_prp P p a d : ty_rec P p a d ty_prp = p.
-  Proof. reflexivity. Qed.
-
-  Theorem ty_rec_arr P p a d A B :
-    ty_rec P p a d (ty_arr A B) =
-    a _ (ty_rec P p a d A) _ (ty_rec P p a d B).
-  Proof. reflexivity. Qed.
-
-  Theorem ty_rec_neq P p a d t :
-    t <> ty_prp -> (forall A B, t <> ty_arr A B) ->
-    ty_rec P p a d t = d t.
-  Proof.
-    intros Np Na. destruct t as [|x y|].
-    - contradiction.
-    - exfalso. now apply (Na x y).
-    - reflexivity.
-  Qed.
-End TyChurch.
-
-Module TyChurchTheories.
-  Module TyTheories := TyTheories TyChurch RlistList.
-  Import TyTheories.
-
-  Notation "'i'" := tyc_obj (in custom stlc_ty at level 0) : stlc_scope.
-
-  (** Examples *)
-  Check -[ o ]-.
-  Check -[ o -> i ]-.
-  Check -[ o -> (i -> o) ]-.
-  Check -[ (o -> i) -> o ]-.
-End TyChurchTheories.
-
-
-(** *** Terms *)
+(*****************)
+(** ** Interface *)
+(*****************)
 
 Declare Custom Entry stlc_tm.
 
-Module Stlc (Ty : TY) (Rlist : RLIST).
+Module Type STLC.
+  Declare Module Ty : TY.
+  Declare Module Rlist : RLIST.
   Module TyTheories := TyTheories Ty Rlist.
   Export TyTheories.
 
-  (** Terms using de Bruijn levels *)
-  Inductive tm : Set :=
-    | tm_lvl : nat -> tm
-    | tm_app : tm -> tm -> tm
-    | tm_abs : ty -> tm -> tm
-    | tm_bot : tm
-    | tm_top : tm
-    | tm_and : tm
-    | tm_or  : tm
-    | tm_imp : tm
-    | tm_for : ty -> tm
-    | tm_ex  : ty -> tm.
+  (** *** Terms *)
+
+  Parameter tm : Set.
+  Parameter tm_lvl : nat -> tm.
+  Parameter tm_app : tm -> tm -> tm.
+  Parameter tm_abs : ty -> tm -> tm.
+
+  Parameter tm_other : tm -> Prop.
+  Axiom tm_other_lvl : forall n, ~ tm_other (tm_lvl n).
+
+  Parameter tm_rect :
+    forall P : tm -> Type,
+    (forall n, P (tm_lvl n)) ->
+    (forall s, P s -> forall t, P t -> P (tm_app s t)) ->
+    (forall T t, P t -> P (tm_abs T t)) ->
+    (forall t, tm_other t -> P t) ->
+    forall t, P t.
+
+  Axiom tm_rect_lvl : forall P l a b o n, tm_rect P l a b o (tm_lvl n) = l n.
+  Axiom tm_rect_app : forall P l a b o s t,
+    tm_rect P l a b o (tm_app s t) = a _ (tm_rect P l a b o s) _ (tm_rect P l a b o t).
+  Axiom tm_rect_abs : forall P l a b o T t,
+    tm_rect P l a b o (tm_abs T t) = b T _ (tm_rect P l a b o t).
+  Axiom tm_rect_other : forall t P l a b o,
+    forall O : tm_other t, tm_rect P l a b o t = o t O.
+
+  (** *** Typing Relation *)
+
+  Parameter has_type : context -> tm -> ty -> Prop.
+
+  Axiom has_type_lvl : forall c n T,
+    has_type c (tm_lvl n) T <-> c !! n = Some T.
+
+  Axiom has_type_app : forall c s t B,
+    has_type c (tm_app s t) B <->
+    exists A, has_type c s (ty_arr A B) /\  has_type c t A.
+
+  Axiom has_type_abs : forall c A T t,
+    has_type c (tm_abs A t) T <->
+    exists B, has_type (c +: A) t B /\ T = -[ A -> B ]-.
+
+  Axiom has_type_other_indep : forall c d t T,
+    tm_other t -> has_type c t T -> has_type d t T.
+
+  Axiom has_type_other_unique : forall c t A B,
+    tm_other t -> has_type c t A -> has_type c t B -> A = B.
+End STLC.
+
+
+(****************)
+(** ** Theories *)
+(****************)
+
+Module StlcTheories (Stlc : STLC).
+  Export Stlc.
+
+
+  (** *** Terms *)
 
   (** Notations *)
-  Notation "<{ x }>" := x (x custom stlc_tm at level 200) : stlc_scope.
-  Notation "x" := x
-    (in custom stlc_tm at level 0, x constr at level 0) : stlc_scope.
-  Notation "( t )" := t
-    (in custom stlc_tm at level 0, t custom stlc_tm) : stlc_scope.
-  Notation "$( x )" := x
-    (in custom stlc_tm at level 0, x constr, only parsing) : stlc_scope.
-  Notation "x y" := (tm_app x y)
-    (in custom stlc_tm at level 10, left associativity) : stlc_scope.
-  Notation "\: A , t" := (tm_abs A t)
-    (in custom stlc_tm at level 200, A custom stlc_ty,
-      t custom stlc_tm at level 200, left associativity) : stlc_scope.
-  Notation "_|" := (tm_bot)
-    (in custom stlc_tm at level 0) : stlc_scope.
-  Notation "^|" := (tm_top)
-    (in custom stlc_tm at level 0) : stlc_scope.
-  Notation "x /\ y" := (tm_and x y)
-    (in custom stlc_tm at level 50, left associativity) : stlc_scope.
-  Notation "x \/ y" := (tm_or x y)
-    (in custom stlc_tm at level 60, left associativity) : stlc_scope.
-  Notation "x > y" := (tm_imp x y)
-    (in custom stlc_tm at level 70, left associativity) : stlc_scope.
-  Notation "'for' T , t" := (tm_app (tm_for T) (tm_abs T t))
-    (in custom stlc_tm at level 200, T custom stlc_ty,
-      t custom stlc_tm at level 200, left associativity) : stlc_scope.
-  Notation "'ex' T , t" := (tm_app (tm_ex T) (tm_abs T t))
-    (in custom stlc_tm at level 200, T custom stlc_ty,
-      t custom stlc_tm at level 200, left associativity) : stlc_scope.
   Coercion tm_lvl : nat >-> tm.
 
+  (** Tactics *)
+  Create HintDb tm.
+  Hint Rewrite tm_rect_lvl tm_rect_app tm_rect_abs : tm.
+  Hint Rewrite tm_rect_other using assumption : tm.
+  Hint Rewrite has_type_lvl has_type_app has_type_abs : tm.
+  Ltac tm_simpl := repeat (simpl in *; autorewrite with tm in *).
+  Ltac tm_simpl1 H := repeat (simpl in H; autorewrite with tm in H).
+  Ltac tm_simplg := repeat (simpl; autorewrite with tm).
 
-  (**************)
-  (** ** Typing *)
-  (**************)
 
-  Inductive has_type : context -> tm -> ty -> Prop :=
-    | t_lvl c n T : c !! n = Some T -> has_type c (tm_lvl n) T
-    | t_app c A B s t : has_type c s (ty_arr A B) -> has_type c t A ->
-        has_type c (tm_app s t) B
-    | t_abs c A B t : has_type (c +: A) t B ->
-        has_type c (tm_abs A t) (ty_arr A B)
-    | t_bot c : has_type c tm_bot ty_prp
-    | t_top c : has_type c tm_top ty_prp
-    | t_and c : has_type c tm_and -[ o -> o -> o ]-
-    | t_or  c : has_type c tm_or  -[ o -> o -> o ]-
-    | t_imp c : has_type c tm_imp -[ o -> o -> o ]-
-    | t_for c T : has_type c (tm_for T) -[ (T -> o) -> o ]-
-    | t_ex  c T : has_type c (tm_ex  T) -[ (T -> o) -> o ]-.
+  Definition tm_rec (P : tm -> Set) := tm_rect P.
+  Definition tm_ind (P : tm -> Prop) := tm_rect P.
 
-  Notation "<| gam |- t : T |>" := (has_type gam t T)
-    (at level 0, gam custom stlc_ty at level 200,
-    t custom stlc_tm, T custom stlc_ty) : stlc_scope.
+  Inductive tmv : Set :=
+    | tmv_lvl : nat -> tmv
+    | tmv_app : tmv -> tmv -> tmv
+    | tmv_abs : ty -> tmv -> tmv
+    | tmv_other : tm -> tmv.
 
-  Fixpoint type_check (c : context) (t : tm) : option ty :=
+  Definition to_tmv : tm -> tmv :=
+    tm_rec _
+      (fun n => tmv_lvl n)
+      (fun s fs t ft => tmv_app fs ft)
+      (fun T t ft => tmv_abs T ft)
+      (fun t _ => tmv_other t).
+
+  Theorem to_tmv_lvl n : to_tmv (tm_lvl n) = tmv_lvl n.
+  Proof. unfold to_tmv. now tm_simpl. Qed.
+
+  Theorem to_tmv_app s t : to_tmv (tm_app s t) = tmv_app (to_tmv s) (to_tmv t).
+  Proof. unfold to_tmv. now tm_simpl. Qed.
+
+  Theorem to_tmv_abs T t : to_tmv (tm_abs T t) = tmv_abs T (to_tmv t).
+  Proof. unfold to_tmv. now tm_simpl. Qed.
+
+  Theorem to_tmv_other t : tm_other t -> to_tmv t = tmv_other t.
+  Proof. intros. unfold to_tmv. now tm_simpl. Qed.
+
+  Hint Rewrite to_tmv_lvl to_tmv_app to_tmv_abs : tm.
+  Hint Rewrite to_tmv_other using assumption : tm.
+
+  Fixpoint to_tm t : tm :=
     match t with
-    | tm_lvl n => c !! n
-    | tm_app s t =>
-        match type_check c s, type_check c t with
-        | Some Ts, Some Tt =>
-            (ty_match None
-              (fun A B => if decide (A = Tt) then Some B else None) None
-            ) Ts
-        | _, _ => None
-        end
-    | tm_abs A t =>
-        match type_check (c +: A) t with
-        | Some B => Some -[ A -> B ]-
-        | _ => None
-        end
-    | tm_bot => Some ty_prp
-    | tm_top => Some ty_prp
-    | tm_and => Some -[ o -> o -> o ]-
-    | tm_or  => Some -[ o -> o -> o ]-
-    | tm_imp => Some -[ o -> o -> o ]-
-    | tm_for T => Some -[ (T -> o) -> o ]-
-    | tm_ex  T => Some -[ (T -> o) -> o ]-
+    | tmv_lvl n => tm_lvl n
+    | tmv_app a b => tm_app (to_tm a) (to_tm b)
+    | tmv_abs T t => tm_abs T (to_tm t)
+    | tmv_other t => t
     end.
 
-  Theorem type_check_sound c t T :
-    type_check c t = Some T -> has_type c t T.
+  Theorem to_tm_to_tmv t : to_tm (to_tmv t) = t.
   Proof.
-    generalize dependent c. generalize dependent T.
-    induction t as [| s IHs t IHt | s t | | | | | | |];
-    intros T c TC; try (simpl in TC; injection TC;
-      intros <-; constructor).
-    - now constructor.
-    - simpl in TC.
-      destruct (type_check c s) as [A|] eqn : Es;
-        [|discriminate].
-      destruct (type_check c t) as [B|] eqn : Et;
-        [|discriminate].
-      unfold ty_match in TC. destruct A as [|X _ Y _ |] using ty_ind;
-        ty_simpl; try discriminate.
-      + destruct (decide (X = B)); [|discriminate].
-        injection TC. intros. subst.
-        econstructor; eauto.
-      + rewrite ty_rec_neq in TC; try assumption.
-        discriminate.
-    - simpl in TC.
-      destruct (type_check (c +: s) t) eqn : E;
-        try discriminate.
-      injection TC. intros <-. constructor.
-      now apply IHt.
+    induction t using tm_ind; unfold to_tmv in *; tm_simpl;
+      unfold to_tmv; congruence.
   Qed.
 
-  Theorem type_check_complete c t T :
-    has_type c t T -> type_check c t = Some T.
-  Proof.
-    generalize dependent c.
-    generalize dependent T.
-    induction t as [| s IHs t IHt | s t | | | | | | |];
-      intros T c TC;
-      inversion TC; subst; try easy; simpl.
-    - erewrite IHs, IHt; try eassumption.
-      unfold ty_match. ty_simpl. now destruct (decide (A = A)).
-    - now erewrite IHt.
-  Qed.
+  Hint Rewrite to_tm_to_tmv : tm.
 
-  Theorem type_check_iff c t T :
-    has_type c t T <-> type_check c t = Some T.
-  Proof.
-    split; intros.
-    - now apply type_check_complete.
-    - now apply type_check_sound.
-  Qed.
+
+  Ltac tmv_f_equal H := apply (f_equal to_tmv) in H; tm_simpl1 H.
+  Ltac tm_discriminate1 H := tmv_f_equal H; discriminate H.
+  Ltac tm_discriminate :=
+    match goal with | [H : _ |- _] => tm_discriminate1 H end.
+  Ltac tm_injection H := tmv_f_equal H; injection H.
+
+
+  (** *** Typing *)
 
   Theorem has_type_unique c t A B :
     has_type c t A -> has_type c t B -> A = B.
   Proof.
-    repeat rewrite type_check_iff.
-    intros -> H. now injection H.
+    generalize dependent B. generalize dependent A.
+    generalize dependent c.
+    induction t using tm_ind; intros c A B HA HB; tm_simpl.
+    - congruence.
+    - destruct HA as (X & HXt1 & HXt2).
+      destruct HB as (Y & HYt1 & HYt2).
+      eapply IHt1 in HXt1; [|eassumption].
+      apply ty_arr_inj in HXt1 as [_ H]. now symmetry.
+    - destruct HA as (X & HXt1 & HXt2).
+      destruct HB as (Y & HYt1 & HYt2).
+      rewrite HXt2, HYt2. f_equal. eapply IHt; eassumption.
+    - eapply has_type_other_unique; eassumption.
   Qed.
 
-
-  (***************************)
-  (** ** Levels manipulation *)
-  (***************************)
-
   (** Apply "f" to all variables in the term "t" *)
-  Fixpoint level_map (f : nat -> nat) (t : tm) : tm :=
-    match t with
-      | tm_lvl n => tm_lvl (f n)
-      | tm_app s t => tm_app (level_map f s) (level_map f t)
-      | tm_abs T t => tm_abs T (level_map f t)
-      | const => const
-    end.
+  Definition level_map (f : nat -> nat) (t : tm) : tm :=
+    (fix fx f x :=
+    match x with
+    | tmv_lvl n => tm_lvl (f n)
+    | tmv_app a b => tm_app (fx f a) (fx f b)
+    | tmv_abs T t => tm_abs T (fx f t)
+    | tmv_other t => t
+    end) f (to_tmv t).
 
   Theorem level_map_f_eq f g t :
     (forall n, f n = g n) -> level_map f t = level_map g t.
   Proof.
-    intros H. induction t; simpl; congruence.
+    intros H. unfold level_map. simpl.
+    induction t using tm_ind; repeat tm_simpl; congruence.
   Qed.
 
   Definition free_level_map f m :=
@@ -513,32 +192,33 @@ Module Stlc (Ty : TY) (Rlist : RLIST).
     generalize dependent T.
     generalize dependent d. generalize dependent c.
     generalize dependent f.
-    induction t as [| | t | | | | | | |];
-    intros f c d L T F HT; inversion HT; subst;
-      unfold free_level_map in *; simpl; try solve [constructor].
+    induction t as [| | t |] using tm_ind; intros f c d T L Hf HT;
+      unfold free_level_map, level_map; tm_simpl.
     - destruct (decide (n < |(c)|)) as [Hn | Hn].
-      + constructor. now rewrite F.
+      + now rewrite Hf.
       + exfalso. apply Hn. apply is_Some_lookup.
         econstructor. eassumption.
-    - econstructor; eauto.
-    - constructor.
-      erewrite level_map_f_eq.
+    - destruct HT as [A [Ht1 Ht2]].
+      exists A. split; eauto.
+    - destruct HT as [B [Hb Ht]].
+      exists B. split; [|assumption].
+      generalize level_map_f_eq. intros E.
+      unfold level_map in E. erewrite E; clear E.
       + apply (IHt (fun n => if decide (n < |(c)|) then f n else n));
           try eassumption; [repeat rewrite rlength_rcons; congruence|].
         intros n.
-        destruct (decide (n < |(c)|)).
-        * repeat rewrite lookup_rcons_lt; try auto.
+        lookup_rcons_spec c t n Hn En; destruct (decide (n < |(c)|)); try lia.
+        * rewrite lookup_rcons_lt; try auto.
           apply is_Some_lookup in l. destruct l.
           eapply is_Some_lookup. econstructor.
-          rewrite F. eassumption.
-        * destruct (decide (n = |(c)|)).
-          -- subst. repeat rewrite lookup_rcons_eq; auto.
-          -- repeat rewrite lookup_None1; try reflexivity;
-               rewrite rlength_rcons; lia.
+          rewrite Hf. eassumption.
+        * subst. rewrite lookup_rcons_eq; auto.
+        * rewrite lookup_None1; try reflexivity; rewrite rlength_rcons; lia.
       + intros n. simpl.
         destruct (decide (n < |(c)|)), (decide (n < |(c +: t)|));
           try reflexivity.
         rewrite rlength_rcons in *. lia.
+    - eapply has_type_other_indep; eassumption.
   Qed.
 
 
@@ -546,55 +226,39 @@ Module Stlc (Ty : TY) (Rlist : RLIST).
   Definition bound_level_map f m :=
     level_map (fun n => if decide (m <= n) then f n else n).
 
-  Theorem has_type_bound_level_map_impl1 l m c d t T :
+  Theorem has_type_bound_level_map_h l m c d t T :
     (l <= |(c)|) ->
     (|(d)| = m + |(c)|) ->
     (forall n, n >= l -> d !! (m + n) = c !! n) ->
     (forall n, n < l -> d !! n = c !! n) ->
-    has_type c t T ->
+    has_type c t T <->
     has_type d (bound_level_map (add m) l t) T.
   Proof.
     generalize dependent T.
     generalize dependent d. generalize dependent c.
-    induction t as [| | t | | | | | | |];
-    intros c d T Hl L Hlg Hll Hc; inversion Hc; subst;
-    unfold bound_level_map in *; simpl; econstructor; try eauto.
+    induction t as [| | t |] using tm_ind;
+    intros c d T Hl L Hlg Hll; unfold bound_level_map, level_map in *; tm_simpl.
     - destruct (decide (l <= n)).
       + now rewrite Hlg.
-      + rewrite Hll; [assumption|lia].
-    - eapply (IHt (c +: t)); try eassumption; try intros n Hn.
-      + rewrite rlength_rcons. lia.
-      + repeat rewrite rlength_rcons. lia.
-      + lookup_rcons_spec c t n Ic Ec; lookup_rcons_spec d t (m + n) Id Ed;
+      + rewrite Hll; [easy|lia].
+    - split; intros (A & H1 & H2); exists A; split;
+        first [eapply IHt1 | eapply IHt2]; eauto.
+    - split; intros (B & Hc & HB); exists B; split; try assumption.
+      + apply (IHt (c +: t)); try assumption; try intros n Hn.
+        * rewrite rlength_rcons. lia.
+        * repeat rewrite rlength_rcons. lia.
+        * lookup_rcons_spec c t n Ic Ec; lookup_rcons_spec d t (m + n) Id Ed;
           try lia; auto.
-      + lookup_rcons_spec c t n Ic Ec; lookup_rcons_spec d t n Id Ed;
-          try lia; auto.
-  Qed.
-
-  Theorem has_type_bound_level_map_impl2 l m c d t T :
-    (l <= |(c)|) ->
-    (|(d)| = m + |(c)|) ->
-    (forall n, n >= l -> d !! (m + n) = c !! n) ->
-    (forall n, n < l -> d !! n = c !! n) ->
-    has_type d (bound_level_map (add m) l t) T
-    ->
-    has_type c t T.
-  Proof.
-    generalize dependent T.
-    generalize dependent d. generalize dependent c.
-    induction t as [| | t | | | | | | |];
-    intros c d T Hl L Hlg Hll Hc; inversion Hc; subst;
-    unfold bound_level_map in *; simpl; econstructor; try eauto.
-    - destruct (decide (l <= n)).
-      + now rewrite <- Hlg.
-      + rewrite <- Hll; [assumption|lia].
-    - eapply (IHt (c +: t)); try eassumption; try intros n Hn.
-      + rewrite rlength_rcons. lia.
-      + repeat rewrite rlength_rcons. lia.
-      + lookup_rcons_spec c t n Ic Ec; lookup_rcons_spec d t (m + n) Id Ed;
-          try lia; auto.
-      + lookup_rcons_spec c t n Ic Ec; lookup_rcons_spec d t n Id Ed;
-          try lia; auto.
+        * lookup_rcons_spec c t n Ic Ec; lookup_rcons_spec d t n Id Ed;
+            try lia; auto.
+      + eapply (IHt (c +: t)); try eassumption; try intros n Hn.
+        * rewrite rlength_rcons. lia.
+        * repeat rewrite rlength_rcons. lia.
+        * lookup_rcons_spec c t n Ic Ec; lookup_rcons_spec d t (m + n) Id Ed;
+            try lia; auto.
+        * lookup_rcons_spec c t n Ic Ec; lookup_rcons_spec d t n Id Ed;
+            try lia; auto.
+    - split; eapply has_type_other_indep; eassumption.
   Qed.
 
   Theorem has_type_bound_level_map1 m c d t T :
@@ -603,7 +267,7 @@ Module Stlc (Ty : TY) (Rlist : RLIST).
     has_type c t T ->
     has_type d (bound_level_map (add m) |(c)| t) T.
   Proof.
-    intros. eapply has_type_bound_level_map_impl1; try eassumption; [lia|].
+    intros. rewrite <- has_type_bound_level_map_h; try eassumption; [lia|].
     intros n Hn. repeat rewrite lookup_None1; auto. lia.
   Qed.
 
@@ -624,7 +288,7 @@ Module Stlc (Ty : TY) (Rlist : RLIST).
     has_type d (bound_level_map (add m) |(c)| t) T ->
     has_type c t T.
   Proof.
-    intros. eapply has_type_bound_level_map_impl2; try eassumption; [lia|].
+    intros. eapply has_type_bound_level_map_h; try eassumption; [lia|].
     intros n Hn. repeat rewrite lookup_None1; auto. lia.
   Qed.
 
@@ -633,14 +297,14 @@ Module Stlc (Ty : TY) (Rlist : RLIST).
   (** ** Substitution *)
   (********************)
 
-  Fixpoint subst m (l : rlist tm) (t : tm) : tm :=
+  Definition subst m l t :=
+    (fix fx m l t :=
     match t with
-    | tm_lvl n => lookup_default (tm_lvl n) n l
-    | tm_app s t => tm_app (subst m l s) (subst m l t)
-    | tm_abs T t =>
-        tm_abs T (subst (S m) ((bound_level_map S m <$> l) +: tm_lvl m) t)
-    | const => const
-    end.
+    | tmv_lvl n => lookup_default (tm_lvl n) n l
+    | tmv_app a b => tm_app (fx m l a) (fx m l b)
+    | tmv_abs T t => tm_abs T (fx (S m) ((bound_level_map S m <$> l) +: tm_lvl m) t)
+    | tmv_other t => t
+    end) m l (to_tmv t).
 
   Theorem has_type_subst_h n Rn (r : rlist tm) (R C : context) (c : ty) :
     |(r)| = |(R)| ->
@@ -657,7 +321,7 @@ Module Stlc (Ty : TY) (Rlist : RLIST).
       rewrite lookup_rcons_lt in H0; [assumption|].
       now rewrite <- L.
     - rewrite lookup_rcons_eq in H; [|now rewrite rlength_fmap].
-      injection H. intros. subst. constructor.
+      injection H. intros. subst. tm_simpl.
       rewrite <- H0.
       repeat rewrite @lookup_rcons_eq; auto.
     - rewrite lookup_rcons_gt in H; [discriminate|now rewrite rlength_fmap].
@@ -671,20 +335,22 @@ Module Stlc (Ty : TY) (Rlist : RLIST).
   Proof.
     generalize dependent r. generalize dependent R.
     generalize dependent T. generalize dependent C.
-    induction t as [| |c ? IH| | | | | | |];
-    simpl; intros C T R r L F HT;
-      inversion HT; subst; try constructor.
+    induction t as [| |c ? IH| ] using tm_ind;
+      simpl; intros C T R r L F HT;
+      unfold subst in *; tm_simpl.
     - unfold lookup_default.
       destruct (r !! n) eqn : E; [now apply (F n) |].
       apply lookup_None2 in E.
-      rewrite @lookup_None1 in H1; [discriminate|].
+      rewrite @lookup_None1 in HT; [discriminate|].
       now rewrite <- L.
-    - econstructor; eauto.
-    - replace (S |(C)|) with (|(C +: c)|); [|apply rlength_rcons].
+    - destruct HT as (A & Ht1 & Ht2). exists A. split; eauto.
+    - destruct HT as (B & H & HB). exists B. split; [|assumption].
+      replace (S |(C)|) with (|(C +: c)|); [|apply rlength_rcons].
       eapply IH; try eassumption.
       + repeat rewrite rlength_rcons. rewrite rlength_fmap.
         now f_equal.
       + intros. eapply has_type_subst_h; eauto.
+    - eapply has_type_other_indep; eassumption.
   Qed.
 
   Theorem has_type_subst2 C T R t r :
@@ -695,32 +361,38 @@ Module Stlc (Ty : TY) (Rlist : RLIST).
   Proof.
     generalize dependent r. generalize dependent R.
     generalize dependent T. generalize dependent C.
-    induction t as [| | t | | | | | | |];
-    simpl; intros C T R r L E F HT;
-      try solve [inversion HT; constructor].
-    - assert (exists A, has_type R n A). {
+    induction t as [| | t |] using tm_ind;
+    simpl; intros C T R r L E F HT.
+    - assert (HT1 := HT). unfold subst in HT; tm_simpl1 HT.
+      assert (exists A, has_type R n A). {
         destruct (decide (n < |(R)|)) as [Hn | Hn].
         - apply is_Some_lookup in Hn as [x Hx].
-          exists x. now constructor.
+          exists x. now tm_simpl.
         - unfold lookup_default in HT.
           rewrite lookup_None1 in HT; [|lia].
-          inversion HT. subst.
-          rewrite @lookup_None1 in H1; [discriminate|lia].
+          tm_simpl.
+          rewrite @lookup_None1 in HT; [discriminate|lia].
       }
       destruct H as [X H]. replace T with X; [assumption|].
       eapply has_type_subst1 in H; try eassumption.
       simpl in H. eapply has_type_unique; eassumption.
-    - inversion HT. subst. econstructor; eauto.
-    - inversion HT. subst. constructor.
+    - unfold subst in *. tm_simpl.
+      destruct HT as (A & Ht1 & Ht2).
+      exists A. split; eauto.
+    - unfold subst in *. tm_simpl.
+      destruct HT as (B & H & HB).
+      exists B. split; [|assumption].
       eapply (IHt (C +: t)).
       4:{
-        replace (S |(C)|) with (|(C +: t)|) in H3; [|rewrite rlength_rcons; lia].
-        apply H3.
+        replace (S |(C)|) with (|(C +: t)|) in H; [|rewrite rlength_rcons; lia].
+        apply H.
       }
       + repeat rewrite rlength_rcons. lia.
       + repeat rewrite rlength_rcons. f_equal.
         now rewrite rlength_fmap.
       + intros. eapply has_type_subst_h; eauto.
+    - unfold subst in HT; tm_simpl.
+      eapply has_type_other_indep; eassumption.
   Qed.
 
 
@@ -738,7 +410,7 @@ Module Stlc (Ty : TY) (Rlist : RLIST).
       destruct (lt_total n |(C)|) as [Ln | [En | Gn]].
       + rewrite @lookup_rcons_lt in H, H0; try assumption.
         * rewrite lookup_build_rlist in H; [|assumption].
-          injection H. intros <-. now constructor.
+          injection H. intros <-. now tm_simpl.
         * now rewrite rlength_build_rlist.
       + rewrite @lookup_rcons_eq in H, H0; try assumption.
         * injection H. injection H0. intros <- <-. assumption.
@@ -746,18 +418,14 @@ Module Stlc (Ty : TY) (Rlist : RLIST).
       + rewrite lookup_rcons_gt in H0; [discriminate|lia].
   Qed.
 
-
-  (*****************)
-  (** ** Reduction *)
-  (*****************)
-
-  Fixpoint level_prop P t : bool :=
+  Definition level_prop P t : bool :=
+    (fix fx P t :=
     match t with
-    | tm_lvl m => P m
-    | tm_abs T s => level_prop P s
-    | tm_app s1 s2 => orb (level_prop P s1) (level_prop P s2)
+    | tmv_lvl m => P m
+    | tmv_abs T s => fx P s
+    | tmv_app s1 s2 => orb (fx P s1) (fx P s2)
     | _ => false
-    end.
+    end) P (to_tmv t).
 
   Definition contains_bound_levels m n :=
     level_prop (fun x => andb (leb m x) (ltb x (n + m))).
@@ -766,36 +434,120 @@ Module Stlc (Ty : TY) (Rlist : RLIST).
     contains_bound_levels m n t = false ->
     bound_level_map (add n) m (bound_level_map (fun x => x - n) m t) = t.
   Proof.
-    unfold bound_level_map, contains_bound_levels. intros L.
-    induction t; try reflexivity; simpl in *.
+    unfold bound_level_map, contains_bound_levels, level_map, level_prop.
+    intros L. induction t using tm_ind; tm_simpl; unfold tm_rec in *.
     - f_equal.
       destruct (decide (m <= n0)), (leb_spec m n0), (ltb_spec n0 (n + m));
         try discriminate; try lia.
       + destruct (decide (m <= n0 - n)); lia.
       + destruct (decide (m <= n0)); lia.
-    - apply orb_false_elim in L. intuition congruence.
+    - apply orb_false_elim in L. unfold tm_rec in *.
+      intuition congruence.
     - intuition congruence.
+    - rewrite (to_tmv_other t0); [|assumption]. now tm_simpl.
   Qed.
 
-  Fixpoint beta_reduction m (t : tm) : tm :=
+  Definition beta_reduction m (t : tm) : tm :=
+    (fix fx m t :=
     match t with
-    | tm_app (tm_abs T t) s =>
-        subst_last m (beta_reduction m s) (beta_reduction (S m) t)
-    | tm_app s t => tm_app (beta_reduction m s) (beta_reduction m t)
-    | tm_abs T t => tm_abs T (beta_reduction (S m) t)
-    | x => x
-    end.
+    | tmv_lvl n => tm_lvl n
+    | tmv_app (tmv_abs T t) s =>
+        subst_last m (fx m s) (fx (S m) t)
+    | tmv_app s t => tm_app (fx m s) (fx m t)
+    | tmv_abs T t => tm_abs T (fx (S m) t)
+    | tmv_other t => t
+    end) m (to_tmv t).
 
-  Fixpoint eta_reduction m (t : tm) {struct t} : tm :=
+  Theorem beta_reduction_app_abs m T t s :
+    beta_reduction m (tm_app (tm_abs T t) s) = subst_last m (beta_reduction m s) (beta_reduction (S m) t).
+  Proof. unfold beta_reduction; now tm_simpl. Qed.
+
+  Theorem beta_reduction_app m s t :
+    (forall A a, s <> tm_abs A a) ->
+    beta_reduction m (tm_app s t) = tm_app (beta_reduction m s) (beta_reduction m t).
+  Proof.
+    intros N.
+    destruct s using tm_ind; unfold beta_reduction; tm_simpl; try reflexivity.
+    exfalso. now eapply N.
+  Qed.
+
+  Theorem beta_reduction_abs m T t :
+    beta_reduction m (tm_abs T t) = tm_abs T (beta_reduction (S m) t).
+  Proof. unfold beta_reduction; now tm_simpl. Qed.
+
+  Theorem beta_reduction_other m t :
+    tm_other t -> beta_reduction m t = t.
+  Proof.
+    intros. unfold beta_reduction. now tm_simpl.
+  Qed.
+
+  Hint Rewrite beta_reduction_app_abs beta_reduction_abs : tm.
+  Hint Rewrite beta_reduction_other using assumption : tm.
+
+
+  Definition eta_reduction m (t : tm) : tm :=
+    (fix fx m t :=
     match t with
-    | tm_abs T (tm_app t (tm_lvl n)) =>
-        if andb (eqb n m) (negb (contains_bound_levels m 1 t)) then
-          bound_level_map (fun x => x - 1) m t
-          else tm_abs T (tm_app (eta_reduction (S m) t) n)
-    | tm_app s t => tm_app (eta_reduction m s) (eta_reduction m t)
-    | tm_abs T t => tm_abs T (eta_reduction (S m) t)
-    | x => x
-    end.
+    | tmv_lvl n => tm_lvl n
+    | tmv_abs T (tmv_app t (tmv_lvl n)) =>
+        if andb (eqb n m) (negb (contains_bound_levels m 1 (to_tm t))) then
+          bound_level_map (fun x => x - 1) m (to_tm t)
+          else tm_abs T (tm_app (fx (S m) t) (tm_lvl n))
+    | tmv_app s t => tm_app (fx m s) (fx m t)
+    | tmv_abs T t => tm_abs T (fx (S m) t)
+    | tmv_other t => t
+    end) m (to_tmv t).
+
+  Theorem eta_reduction_lvl m n:
+    eta_reduction m (tm_lvl n) = tm_lvl n.
+  Proof. unfold eta_reduction; now tm_simpl. Qed.
+
+  Theorem eta_reduction_app m s t :
+    eta_reduction m (tm_app s t) = tm_app (eta_reduction m s) (eta_reduction m t).
+  Proof. unfold eta_reduction; now tm_simpl. Qed.
+
+  Theorem eta_reduction_abs_app m T t:
+    contains_bound_levels m 1 t = false ->
+    eta_reduction m (tm_abs T (tm_app t (tm_lvl m))) =
+    bound_level_map (fun x => x - 1) m t.
+  Proof.
+    intros.
+    unfold eta_reduction. tm_simpl.
+    rewrite eqb_refl. now rewrite H.
+  Qed.
+
+  Theorem eta_reduction_abs_app2 m t T :
+    contains_bound_levels m 1 t = true ->
+    eta_reduction m (tm_abs T (tm_app t (tm_lvl m))) =
+    tm_abs T (tm_app (eta_reduction (S m) t) (tm_lvl m)).
+  Proof.
+    intros. unfold eta_reduction. tm_simpl.
+    rewrite eqb_refl. now rewrite H.
+  Qed.
+
+  Theorem eta_reduction_abs_app3 m n t T :
+    n <> m ->
+    eta_reduction m (tm_abs T (tm_app t (tm_lvl n))) =
+    tm_abs T (tm_app (eta_reduction (S m) t) (tm_lvl n)).
+  Proof.
+    intros. unfold eta_reduction. tm_simpl.
+    destruct (eqb_spec n m); [lia|].
+    reflexivity.
+  Qed.
+
+  Theorem eta_reduction_abs m T t :
+    (forall a, t <> tm_app a (tm_lvl m)) ->
+    eta_reduction m (tm_abs T t) = tm_abs T (eta_reduction (S m) t).
+  Proof.
+    intros N.
+    destruct t using tm_ind; unfold eta_reduction; tm_simpl; try reflexivity.
+    destruct t2 using tm_ind; tm_simpl; try reflexivity.
+    destruct (eqb_spec n m).
+    - subst. exfalso. now eapply N.
+    - auto.
+  Qed.
+
+  Hint Rewrite eta_reduction_app : tm.
 
 
   Theorem has_type_beta_reduction C T t :
@@ -803,18 +555,27 @@ Module Stlc (Ty : TY) (Rlist : RLIST).
     has_type C (beta_reduction |(C)| t) T.
   Proof.
     generalize dependent T. generalize dependent C.
-    induction t; intros C T HT; try assumption.
-    - destruct t1; try solve
-        [inversion HT; subst; econstructor; eauto].
-      inversion HT. subst.
-      simpl. eapply has_type_subst_last; [|eauto].
-      apply IHt1 in H2. simpl in H2. inversion H2. subst.
-      apply ty_arr_inj in H5. destruct H5. now subst.
-    - inversion HT. subst.
-      simpl. constructor.
-      specialize IHt with (C +: t0) B.
-      rewrite rlength_rcons in IHt.
-      auto.
+    induction t using tm_ind; intros C A HT.
+    - unfold beta_reduction; now tm_simpl.
+    - tm_simpl. destruct HT as (B & Ht1 & Ht2).
+      assert (D : (forall T t, t1 <> tm_abs T t) \/ exists T t, t1 = tm_abs T t). {
+        destruct t1 using tm_ind; try (left; intros * ?; tm_discriminate).
+        right. eauto.
+      }
+      destruct D.
+      + rewrite beta_reduction_app; [|auto].
+        tm_simplg. exists B. split; auto.
+      + destruct H as (T & t & Ht). subst. tm_simplg.
+        eapply has_type_subst_last; [|eauto].
+        apply IHt1 in Ht1 as F. tm_simpl.
+        destruct F as (D & HD1 & HD2).
+        apply ty_arr_inj in HD2. destruct HD2. now subst.
+    - tm_simpl.
+      destruct HT as (B & HB1 & HB2).
+      eexists. split; [|eassumption].
+      replace (S |(C)|) with |(C +: T)|; [|now rewrite rlength_rcons].
+      now apply IHt.
+    - now tm_simpl.
   Qed.
 
   Theorem has_type_eta_reduction C T t :
@@ -822,58 +583,43 @@ Module Stlc (Ty : TY) (Rlist : RLIST).
     has_type C (eta_reduction |(C)| t) T.
   Proof.
     generalize dependent T. generalize dependent C.
-    induction t; intros C T HT; try assumption;
-    inversion HT; subst; try solve [econstructor; eauto].
-    assert (IH := IHt (C +: t0)). rewrite rlength_rcons in IH.
-    destruct t1; try solve [econstructor; eauto].
-    simpl in IH.
-    destruct t1_2; try solve [constructor; auto]. simpl.
-    destruct (eqb_spec n |(C)|);
-    destruct (contains_bound_levels |(C)| 1 t1_1) eqn : E;
-      try solve [constructor; auto].
-    simpl in *. inversion H3. subst.
-    inversion H5. subst.
-    rewrite @lookup_rcons_eq in H1; [|lia].
-    injection H1. intros ->.
-    eapply has_type_bound_level_map2.
-    3:{ rewrite bound_level_map_id; eassumption. }
-    - now rewrite rlength_rcons.
-    - intros. now rewrite lookup_rcons_lt.
+    induction t using tm_ind; intros C A HT.
+    - unfold eta_reduction; now tm_simpl.
+    - tm_simpl. destruct HT as (B & HB1 & HB2).
+      exists B. split; auto.
+    - tm_simpl. destruct HT as (B & HB1 & HB2).
+      assert (D : (forall a n, t0 <> tm_app a (tm_lvl n)) \/ exists a n, t0 = tm_app a (tm_lvl n)). {
+        destruct t0 using tm_ind; try (left; intros * ?; tm_discriminate).
+        destruct t0_2 using tm_ind; try (left; intros * ?; tm_discriminate).
+        - right. eauto.
+        - left. intros * N. tm_injection N. intros.
+          apply (f_equal to_tm) in H0. tm_simpl. tm_discriminate.
+      }
+      destruct D.
+      + rewrite eta_reduction_abs; [|auto].
+        tm_simplg. exists B. split; [|assumption].
+        apply IHt in HB1. now rewrite rlength_rcons in HB1.
+      + destruct H as (a & n & Ha). subst.
+        destruct (eqb_spec n |(C)|).
+        * subst.
+          destruct (contains_bound_levels |(C)| 1 a) eqn : E.
+          -- rewrite eta_reduction_abs_app2; [|assumption].
+             tm_simplg. exists B. split; [|reflexivity].
+             apply IHt in HB1. rewrite rlength_rcons in HB1.
+             now rewrite eta_reduction_app, eta_reduction_lvl in HB1.
+          -- rewrite eta_reduction_abs_app; [|assumption].
+             apply (has_type_bound_level_map2 1 _ (C +: T)).
+             ++ now rewrite rlength_rcons.
+             ++ intros n Hn. lookup_rcons_spec C T n H F; try reflexivity; lia.
+             ++ tm_simpl1 HB1.
+                rewrite bound_level_map_id; auto.
+                destruct HB1 as (A & HA1 & HA2).
+                tm_simpl. rewrite @lookup_rcons_eq in HA2; [|reflexivity].
+                injection HA2. now intros ->.
+        * rewrite eta_reduction_abs_app3; [|assumption].
+          tm_simplg. exists B. split; [|reflexivity].
+           apply IHt in HB1. rewrite rlength_rcons in HB1.
+           now rewrite eta_reduction_app, eta_reduction_lvl in HB1.
+    - unfold eta_reduction. now tm_simpl.
   Qed.
-End Stlc.
-
-
-(****************)
-(** ** Examples *)
-(****************)
-
-Module StlcChurch.
-  Module Stlc := Stlc TyChurch RlistList.
-  Import Stlc.
-  Import TyChurchTheories.
-
-  (** Terms *)
-  Check <{ \: i, 0 }>.
-  Check <{ (\: (i -> o), 2) 1 }>.
-  Check <{ \: o, 3 _| }>.
-
-  (** Typing *)
-  Compute type_check [-[ i -> o ]-; tyc_obj] <{ 0 1 }>.
-
-  (** Substitution *)
-  Compute subst 1 [<{ \: i, 1 }>; tm_lvl 0] <{ \: o, 1 0 }>.
-  Compute subst 2 [<{ \: i, 1 }>; tm_lvl 0] <{ \: o, 1 0 }>.
-  Compute subst 2 [<{ \: i, 0 1 }>] <{ \: o, 0 }>.
-  Compute subst 1 [<{ \: i, 0 1 }>] <{ \: o, 0 }>.
-  Compute subst 0 [<{ \: i, 0 0 }>] <{ \: o, 0 }>.
-  Compute subst 4 [tm_lvl 0; <{ \: i, 5 }>; tm_lvl 2] <{ 1 2 }>.
-  Compute subst 2 [tm_lvl 0; <{ \: i, 1 2 }>] <{ \: o, 1 }>.
-  Compute subst 0 [tm_lvl 0; tm_lvl 1; <{ \: i, 0 0 }>] <{ \: o, \: i, 2 2 }>.
-  Compute subst 0 [ tm_top ] <{ \: o, 1 }>.
-  Compute subst_last 1 tm_bot <{ \: o, 1 }>.
-
-  (** Reduction *)
-  Compute beta_reduction 1 <{ (\: o, 1) 0 }>.
-  Compute beta_reduction 0 <{ (\: o -> o, 0) (\: o, 0) }>.
-  Compute beta_reduction 0 <{ (\: o -> o, 0) ((\: o -> o, 0) (\: o, 0)) }>.
-End StlcChurch.
+End StlcTheories.
